theories/typing/array.v
@@ -1,0 +1,49 @@
+Require Import FunctionalExtensionality Equality.
+From iris.proofmode Require Import tactics.
+From lrust.util Require Import basic types.
+From lrust.typing Require Import product mod_ty.
+From lrust.typing Require Export type.
+Set Default Proof Using "Type".
+
+Section array.
+  Context `{!typeG Σ}.
+
+  Fixpoint array {A} n (ty: type A) : type (pvec A n) :=
+    match n with 0 => <{const -[] }> unit_ty |
+      S m => <{curry (-::)}> (ty * array m ty) end.
+
+  Global Instance array_ne {A} n : NonExpansive (@array A n).
+  Proof. elim n=>/=; [apply _|]. by move=> ?????->. Qed.
+
+  Global Instance array_type_ne {A} n : TypeNonExpansive (@array A n).
+  Proof. elim n=>/=; apply _. Qed.
+
+  Global Instance array_copy {A} n (ty: _ A) : Copy ty → Copy (array n ty).
+  Proof. move=> ?. elim n=>/=; apply _. Qed.
+  Global Instance array_send {A} n (ty: _ A) : Send ty → Send (array n ty).
+  Proof. move=> ?. elim n=>/=; apply _. Qed.
+  Global Instance array_sync {A} n (ty: _ A) : Sync ty → Sync (array n ty).
+  Proof. move=> ?. elim n=>/=; apply _. Qed.
+
+  Lemma array_plus_prod {A} E L m n (ty: _ A) :
+    eqtype E L pvsep (curry pvapp) (array (m + n) ty) (array m ty * array n ty).
+  Proof.
+    elim: m=> [|m Eq].
+    - have [->->]: @pvsep A 0 n = prod_map (const -[]) id ∘ prod_left_id' ∧
+        curry (@pvapp A 0 n) = prod_left_id ∘ prod_map (const ()) id.
+      { split; extensionality x; by [case x=> [[]?]|]. }
+      eapply eqtype_trans; [apply eqtype_symm; apply prod_ty_left_id|].
+      apply prod_eqtype; [|done].
+      apply mod_ty_inout, functional_extensionality. by move=> [].
+    - have [->->]: @pvsep A (S m) n = prod_map prod_to_cons_prod id ∘
+          prod_assoc ∘ prod_map id pvsep ∘ cons_prod_to_prod ∧
+        curry (@pvapp A (S m) n) = prod_to_cons_prod ∘
+          (prod_map id (curry pvapp) ∘ (prod_assoc' ∘ prod_map cons_prod_to_prod id)).
+      { split; extensionality x; [|by case x=> [[??]?]]. case x=> [? xl]/=.
+        by case (pvsep xl). }
+      eapply eqtype_trans. { apply mod_ty_outin, _. } eapply eqtype_trans.
+      { apply prod_eqtype; [done|apply Eq]. } eapply eqtype_trans.
+      { apply prod_ty_assoc. } apply prod_eqtype; [apply mod_ty_inout, _|done].
+  Qed.
+
+End array.
